coq/proof/SoundForgetMemory.v
@@ -29,14 +29,9 @@ Require Import SoundForget.
 Set Implicit Arguments.
 
 
-Definition noalias_with_def_memory (conf:Config) (def_memory:option (GenericValue * typ)) (ptr:GenericValue) (ty:typ): Prop :=
-  forall gptr_def ty_def
-         (DEF: def_memory = Some (gptr_def, ty_def)),
-    InvState.Unary.sem_noalias conf gptr_def ptr ty_def ty.
-
 Inductive mem_change : Type :=
 | mem_change_alloc
-    (gsz:sz) (gn:GenericValue) (a:align)
+    (def_var:id) (b:mblock) (ty:typ) (s:sz) (gn:GenericValue) (a:align)
 | mem_change_store
     (ptr:GenericValue) (ty:typ) (gv:GenericValue) (a:align)
 | mem_change_free
@@ -44,23 +39,18 @@ Inductive mem_change : Type :=
 | mem_change_none
 .
 
-(* Definition ptr_to_genericvalue conf st invst ptr: option (GenericValue * typ) := *)
-(*   match InvState.Unary.sem_valueT conf st invst ptr.(fst) with *)
-(*   | Some gv => Some (gv, ptr.(snd)) *)
-(*   | None => None *)
-(*   end. *)
-
-Inductive mem_change_inject conf_src conf_tgt invmem: mem_change -> mem_change -> Prop :=
+Inductive mem_change_inject (conf_src conf_tgt:Config) invmem: mem_change -> mem_change -> Prop :=
 | mem_change_inject_alloc_alloc
     gsz gn0 gn1 a
+    b_src b_tgt ty dv
     (N_INJECT: genericvalues_inject.gv_inject invmem.(InvMem.Rel.inject) gn0 gn1)
-  : mem_change_inject conf_src conf_tgt invmem (mem_change_alloc gsz gn0 a) (mem_change_alloc gsz gn1 a)
+  : mem_change_inject conf_src conf_tgt invmem (mem_change_alloc dv b_src ty gsz gn0 a) (mem_change_alloc dv b_tgt ty gsz gn1 a)
 | mem_change_inject_alloc_none
-    gsz gn a
-  : mem_change_inject conf_src conf_tgt invmem (mem_change_alloc gsz gn a) mem_change_none
+    gsz gn a b ty dv
+  : mem_change_inject conf_src conf_tgt invmem (mem_change_alloc dv b ty gsz gn a) mem_change_none
 | mem_change_inject_none_alloc
-    gsz gn a
-  : mem_change_inject conf_src conf_tgt invmem mem_change_none (mem_change_alloc gsz gn a)
+    gsz gn a b ty dv
+  : mem_change_inject conf_src conf_tgt invmem mem_change_none (mem_change_alloc dv b ty gsz gn a)
 | mem_change_inject_store_store
     ptr0 ptr1 gv0 gv1 ty a
     (PTR_INJECT: genericvalues_inject.gv_inject invmem.(InvMem.Rel.inject) ptr0 ptr1)
@@ -68,7 +58,7 @@ Inductive mem_change_inject conf_src conf_tgt invmem: mem_change -> mem_change -
   : mem_change_inject conf_src conf_tgt invmem (mem_change_store ptr0 ty gv0 a) (mem_change_store ptr1 ty gv1 a)
 | mem_change_inject_store_nop
     ptr gv ty a b ofs
-    (GV2PTR: GV2ptr conf_src.(CurTargetData) (getPointerSize conf_tgt.(CurTargetData)) ptr = Some (Values.Vptr b ofs))
+    (GV2PTR: GV2ptr conf_src.(CurTargetData) (getPointerSize conf_src.(CurTargetData)) ptr = Some (Values.Vptr b ofs))
     (IN: In b invmem.(InvMem.Rel.src).(InvMem.Unary.private))
   : mem_change_inject conf_src conf_tgt invmem (mem_change_store ptr ty gv a) mem_change_none
 | mem_change_inject_free
@@ -79,112 +69,451 @@ Inductive mem_change_inject conf_src conf_tgt invmem: mem_change -> mem_change -
     : mem_change_inject conf_src conf_tgt invmem mem_change_none mem_change_none
 .
 
-(* Inductive mem_change_rel conf st: mem_change -> cmd -> Prop := *)
-(* | mem_change_rel_alloca *)
-(*     id ty v *)
-(*     tsz gn a *)
-(*     (TYPE: getTypeAllocSize conf.(CurTargetData) ty = Some tsz) *)
-(*     (VAL: getOperandValue conf.(CurTargetData) v st.(EC).(Locals) conf.(Globals)) *)
-(*   : mem_change_rel conf st (mem_change_alloc tsz gn a) (insn_alloca id ty v a) *)
-(* | mem_change_rel_malloc *)
-(*     id ty v *)
-(*     tsz gn a *)
-(*     (TYPE: getTypeAllocSize conf.(CurTargetData) ty = Some tsz) *)
-(*     (VAL: getOperandValue conf.(CurTargetData) v st.(EC).(Locals) conf.(Globals)) *)
-(*   : mem_change_rel conf st (mem_change_alloc tsz gn a) (insn_malloc id ty v a) *)
-(* | mem_change_rel_store *)
-(*     v_val gv_val *)
-(*     v_ptr gv_ptr *)
-(*     ty a sid *)
-(*     (VAL: getOperandValue conf.(CurTargetData) v_val st.(EC).(Locals) conf.(Globals) = Some gv_val) *)
-(*     (PTR: getOperandValue conf.(CurTargetData) v_ptr st.(EC).(Locals) conf.(Globals) = Some gv_ptr) *)
-(*   : mem_change_rel conf st (mem_change_store gv_ptr ty gv_val a) *)
-(*                    (insn_store sid ty v_val v_ptr a) *)
-(* | mem_change_rel_free *)
-(*     v_ptr gv_ptr fid ty *)
-(*     (PTR: getOperandValue conf.(CurTargetData) v_ptr st.(EC).(Locals) conf.(Globals) = Some gv_ptr) *)
-(*   : mem_change_rel conf st (mem_change_free gv_ptr) (insn_free fid ty v_ptr). *)
-(* | mem_change_rel_none *)
-(*     cmd *)
-(*     (NON_ALLOCA =  *)
-(*   : mem_change_rel conf st mem_change_none cmd *)
-
-Definition mem_change_rel conf st mc cmd: Prop :=
-  match cmd with
-  | insn_alloca _ ty v a =>
-    exists tsz gn,
-    <<TYPE: getTypeAllocSize conf.(CurTargetData) ty = Some tsz>> /\
-    <<VAL: getOperandValue conf.(CurTargetData) v st.(EC).(Locals) conf.(Globals) = Some gn>> /\
-    <<MEM_CH: mc = mem_change_alloc tsz gn a>>
-  | insn_malloc _ ty v a =>
-    exists tsz gn,
-    <<TYPE: getTypeAllocSize conf.(CurTargetData) ty = Some tsz>> /\
-    <<VAL: getOperandValue conf.(CurTargetData) v st.(EC).(Locals) conf.(Globals) = Some gn>> /\
-    <<MEM_CH: mc = mem_change_alloc tsz gn a>>
-  | insn_store _ ty v_val v_ptr a =>
-    exists gv_val gv_ptr,
-    <<VAL: getOperandValue conf.(CurTargetData) v_val st.(EC).(Locals) conf.(Globals) = Some gv_val>> /\
-    <<PTR: getOperandValue conf.(CurTargetData) v_ptr st.(EC).(Locals) conf.(Globals) = Some gv_ptr>> /\
-    <<MEM_CH: mc = mem_change_store gv_ptr ty gv_val a>>
-  | insn_free _ _ v_ptr =>
-    exists gv_ptr,
-    <<PTR: getOperandValue conf.(CurTargetData) v_ptr st.(EC).(Locals) conf.(Globals) = Some gv_ptr>> /\
-    <<MEM_CH: mc = mem_change_free gv_ptr>>
-  | _ => mc = mem_change_none
-  end.
-
-Definition mem_change_rel2 conf st mc cmd: Prop :=
-  match cmd with
-  | insn_alloca _ ty v a =>
-    exists tsz gn,
-    <<MEM_CH: mc = mem_change_alloc tsz gn a>>
-  | insn_malloc _ ty v a =>
-    exists tsz gn,
-    <<MEM_CH: mc = mem_change_alloc tsz gn a>>
-  | insn_store _ ty _ v_ptr a =>
-    exists gv_val gv_ptr,
-    <<PTR: getOperandValue conf.(CurTargetData) v_ptr st.(EC).(Locals) conf.(Globals) = Some gv_ptr>> /\
-    <<MEM_CH: mc = mem_change_store gv_ptr ty gv_val a>>
-  | insn_free _ _ v_ptr =>
-    exists gv_ptr,
-    <<PTR: getOperandValue conf.(CurTargetData) v_ptr st.(EC).(Locals) conf.(Globals) = Some gv_ptr>> /\
-    <<MEM_CH: mc = mem_change_free gv_ptr>>
-  | _ => mc = mem_change_none
-  end.
-
-Inductive mem_change_equiv (conf:Config) (mem0 mem1:mem): mem_change -> Prop :=
-| mem_change_equiv_alloc
-    mb bsz gn a
-    (MALLOC: Some (mem1, mb) = malloc conf.(CurTargetData) mem0 bsz gn a)
-  : mem_change_equiv conf mem0 mem1 (mem_change_alloc bsz gn a)
-| mem_change_equiv_store
+Inductive states_mem_change (conf:Config) (st0 st1:State): mem_change -> Prop :=
+| states_mem_change_alloc
+    mb ty bsz gn a dv
+    (MALLOC: Some (st1.(Mem), mb) = malloc conf.(CurTargetData) st0.(Mem) bsz gn a)
+    (UNIQUE: InvState.Unary.sem_unique conf st0 dv)
+    (DEF_VAR: lookupAL _ st1.(EC).(Locals) dv = Some (blk2GV conf.(CurTargetData) mb))
+  : states_mem_change conf st0 st1 (mem_change_alloc dv mb ty bsz gn a)
+| states_mem_change_store
     ptr ty gv a
-    (STORE: Some mem1 = mstore conf.(CurTargetData) mem0 ptr ty gv a)
-  : mem_change_equiv conf mem0 mem1 (mem_change_store ptr ty gv a)
-| mem_change_equiv_free
+    (STORE: Some st1.(Mem) = mstore conf.(CurTargetData) st0.(Mem) ptr ty gv a)
+  : states_mem_change conf st0 st1 (mem_change_store ptr ty gv a)
+| states_mem_change_free
     ptr
-    (FREE: Some mem1 = free conf.(CurTargetData) mem0 ptr)
-  : mem_change_equiv conf mem0 mem1 (mem_change_free ptr)
-| mem_change_equiv_none
-    (MEM_EQ: mem0 = mem1)
-  : mem_change_equiv conf mem0 mem1 mem_change_none
+    (FREE: Some st1.(Mem) = free conf.(CurTargetData) st0.(Mem) ptr)
+  : states_mem_change conf st0 st1 (mem_change_free ptr)
+| states_mem_change_none
+    (MEM_EQ: st0.(Mem) = st1.(Mem))
+  : states_mem_change conf st0 st1 mem_change_none
 .
 
 Inductive state_equiv_except_mem (conf:Config) (st0 st1:State) (mem_chng:mem_change) :=
 | state_equiv_except_mem_intro
     (LOCALS_EQ: st0.(EC).(Locals) = st1.(EC).(Locals))
-    (MEM_CHANGE_EQUIV: mem_change_equiv conf st0.(Mem) st1.(Mem) mem_chng)
+    (STATES_MEM_CHANGE: states_mem_change conf st0 st1 mem_chng)
 .
+
+(* proof for private_parent *)
+
+Definition mem_change_no_private_parent conf mc pp: Prop :=
+  match mc with
+  | mem_change_store ptr _ _ _
+  | mem_change_free ptr =>
+    forall b ofs
+           (PTR: GV2ptr conf.(CurTargetData) conf.(CurTargetData).(getPointerSize) ptr =
+                 Some (Values.Vptr b ofs)),
+      ~ In b pp
+  | _ => True
+  end.
+
+Lemma gv_inject_ptr_public_src
+      invmem ptr0 ptr1 b ofs conf_src
+      (PTR_INJECT : genericvalues_inject.gv_inject (InvMem.Rel.inject invmem) ptr0 ptr1)
+      (PTR : GV2ptr (CurTargetData conf_src) (getPointerSize (CurTargetData conf_src)) ptr0 = Some (Values.Vptr b ofs))
+  : InvMem.Rel.public_src (InvMem.Rel.inject invmem) b.
+Proof.
+  exploit genericvalues_inject.simulation__GV2ptr; try exact PTR; eauto. i. des.
+  ii. inv x1. clarify.
+Qed.
+
+Lemma mem_change_inject_no_private_parent_src
+      conf_src mc_src mem_src
+      conf_tgt mc_tgt mem_tgt
+      invmem
+      (SEM: InvMem.Rel.sem conf_src conf_tgt mem_src mem_tgt invmem)
+      (INJECT: mem_change_inject conf_src conf_tgt invmem mc_src mc_tgt)
+  : mem_change_no_private_parent conf_src mc_src invmem.(InvMem.Rel.src).(InvMem.Unary.private_parent).
+Proof.
+  inv SEM.
+  inv SRC.
+  inv INJECT; try econs; ii.
+  - exploit PRIVATE_PARENT; eauto. i. des.
+    hexploit gv_inject_ptr_public_src; try apply PTR; eauto.
+  - rewrite PTR in GV2PTR. clarify.
+    exploit PRIVATE; eauto. i. des.
+    exploit DISJOINT; eauto.
+  - exploit PRIVATE_PARENT; eauto. i. des.
+    hexploit gv_inject_ptr_public_src; try apply PTR; eauto.
+Qed.
+
+Lemma simulation__GV2ptr_tgt
+     : forall (mi : Values.meminj) (TD : TargetData) (gv1 gv1' : GenericValue) (v' : Values.val),
+       genericvalues_inject.gv_inject mi gv1 gv1' ->
+       GV2ptr TD (getPointerSize TD) gv1' = Some v' ->
+       exists v : Values.val, GV2ptr TD (getPointerSize TD) gv1 = Some v /\ memory_sim.MoreMem.val_inject mi v v'.
+Proof.
+  i.
+  unfold GV2ptr in *.
+  destruct gv1'; clarify.
+  destruct p. destruct v; clarify.
+  destruct gv1'; clarify.
+  destruct gv1; inv H.
+  destruct v1; inv H3.
+  inv H6.
+  esplits; eauto.
+Qed.
+
+Lemma gv_inject_ptr_public_tgt
+      ptr_src
+      ptr_tgt conf_tgt b_tgt ofs_tgt
+      invmem
+      (PTR_INJECT : genericvalues_inject.gv_inject (InvMem.Rel.inject invmem) ptr_src ptr_tgt)
+      (PTR_TGT : GV2ptr (CurTargetData conf_tgt) (getPointerSize (CurTargetData conf_tgt)) ptr_tgt = Some (Values.Vptr b_tgt ofs_tgt))
+  : InvMem.Rel.public_tgt (InvMem.Rel.inject invmem) b_tgt.
+Proof.
+  exploit simulation__GV2ptr_tgt; try exact PTR_TGT; eauto. i. des.
+  inv x1. unfold InvMem.Rel.public_tgt. esplits; eauto.
+Qed.
+
+Lemma mem_change_inject_no_private_parent_tgt
+      conf_src mc_src mem_src
+      conf_tgt mc_tgt mem_tgt
+      invmem
+      (SEM: InvMem.Rel.sem conf_src conf_tgt mem_src mem_tgt invmem)
+      (INJECT: mem_change_inject conf_src conf_tgt invmem mc_src mc_tgt)
+  : mem_change_no_private_parent conf_tgt mc_tgt invmem.(InvMem.Rel.tgt).(InvMem.Unary.private_parent).
+Proof.
+  inv SEM.
+  inv TGT.
+  inv INJECT; try econs; ii.
+  - exploit PRIVATE_PARENT; eauto. i. des.
+    hexploit gv_inject_ptr_public_tgt; try apply PTR; eauto.
+  - exploit PRIVATE_PARENT; eauto. i. des.
+    hexploit gv_inject_ptr_public_tgt; try apply PTR; eauto.
+Qed.
+
+(* Difference btw rel and rel_after: changing locals & forget *)
+
+Definition mem_change_cmd conf st mc cmd: Prop :=
+  match cmd with
+  | insn_alloca dv ty v a =>
+    exists mb tsz gn,
+    <<TYPE: getTypeAllocSize conf.(CurTargetData) ty = Some tsz>> /\
+    <<VAL: getOperandValue conf.(CurTargetData) v st.(EC).(Locals) conf.(Globals) = Some gn>> /\
+    <<MEM_CH: mc = mem_change_alloc dv mb ty tsz gn a>>
+  | insn_malloc dv ty v a =>
+    exists mb tsz gn,
+    <<TYPE: getTypeAllocSize conf.(CurTargetData) ty = Some tsz>> /\
+    <<VAL: getOperandValue conf.(CurTargetData) v st.(EC).(Locals) conf.(Globals) = Some gn>> /\
+    <<MEM_CH: mc = mem_change_alloc dv mb ty tsz gn a>>
+  | insn_store _ ty v_val v_ptr a =>
+    exists gv_val gv_ptr,
+    <<VAL: getOperandValue conf.(CurTargetData) v_val st.(EC).(Locals) conf.(Globals) = Some gv_val>> /\
+    <<PTR: getOperandValue conf.(CurTargetData) v_ptr st.(EC).(Locals) conf.(Globals) = Some gv_ptr>> /\
+    <<MEM_CH: mc = mem_change_store gv_ptr ty gv_val a>>
+  | insn_free dv _ v_ptr =>
+    exists gv_ptr,
+    <<PTR: getOperandValue conf.(CurTargetData) v_ptr st.(EC).(Locals) conf.(Globals) = Some gv_ptr>> /\
+    <<MEM_CH: mc = mem_change_free gv_ptr>>
+  | _ => mc = mem_change_none
+  end.
+
+Definition mem_change_cmd_after conf st mc cmd inv0: Prop :=
+  match cmd with
+  | insn_alloca dv ty v a =>
+    exists mb tsz gn,
+    <<TYPE: getTypeAllocSize conf.(CurTargetData) ty = Some tsz>> /\
+    (* <<VAL: getOperandValue conf.(CurTargetData) v st.(EC).(Locals) conf.(Globals) = Some gn>> /\ *)
+    <<FORGET: inv_unary_forgot inv0 (AtomSetImpl.singleton dv)>> /\
+    <<MEM_CH: mc = mem_change_alloc dv mb ty tsz gn a>>
+  | insn_malloc dv ty v a =>
+    exists mb tsz gn,
+    <<TYPE: getTypeAllocSize conf.(CurTargetData) ty = Some tsz>> /\
+    (* <<VAL: getOperandValue conf.(CurTargetData) v st.(EC).(Locals) conf.(Globals) = Some gn>> /\ *)
+    <<FORGET: inv_unary_forgot inv0 (AtomSetImpl.singleton dv)>> /\
+    <<MEM_CH: mc = mem_change_alloc dv mb ty tsz gn a>>
+  | insn_store _ ty v_val v_ptr a =>
+    exists gv_val gv_ptr,
+    <<VAL: getOperandValue conf.(CurTargetData) v_val st.(EC).(Locals) conf.(Globals) = Some gv_val>> /\
+    <<PTR: getOperandValue conf.(CurTargetData) v_ptr st.(EC).(Locals) conf.(Globals) = Some gv_ptr>> /\
+    <<MEM_CH: mc = mem_change_store gv_ptr ty gv_val a>>
+  | insn_free dv _ v_ptr =>
+    exists gv_ptr,
+    <<PTR: getOperandValue conf.(CurTargetData) v_ptr st.(EC).(Locals) conf.(Globals) = Some gv_ptr>> /\
+    <<MEM_CH: mc = mem_change_free gv_ptr>>
+  | _ => mc = mem_change_none
+  end.
 
 Definition unique_preserved_mem conf st inv: Prop :=
   forall u (MEM: AtomSetImpl.mem u inv.(Invariant.unique) = true),
     InvState.Unary.sem_unique conf st u.
 
-(* Definition ptr_to_genericvalue conf st invst ptr: option (GenericValue * typ) := *)
-(*   match InvState.Unary.sem_valueT conf st invst ptr.(fst) with *)
-(*   | Some gv => Some (gv, ptr.(snd)) *)
-(*   | None => None *)
-(*   end. *)
+(* Subset *)
+
+Lemma forget_memory_unary_Subset
+      def_mem inv0
+  : Invariant.Subset_unary (ForgetMemory.unary def_mem inv0) inv0.
+Proof.
+  unfold ForgetMemory.unary.
+  econs; ss; ii; des_ifs; try econs; ss.
+  eapply ExprPairSetFacts.filter_iff in H; try by solve_compat_bool.
+  des. eauto.
+Qed.
+
+Lemma forget_memory_Subset
+      def_mem_src def_mem_tgt  inv0
+  : Invariant.Subset (ForgetMemory.t def_mem_src def_mem_tgt inv0) inv0.
+Proof.
+  unfold ForgetMemory.t; des_ifs;
+    econs; ss; try reflexivity; apply forget_memory_unary_Subset.
+Qed.
+
+(* specs for equiv_except *)
+
+Lemma sem_idT_eq_locals
+      st0 st1 invst0 x
+      (LOCALS_EQ : Locals (EC st0) = Locals (EC st1))
+  : InvState.Unary.sem_idT st0 invst0 x = InvState.Unary.sem_idT st1 invst0 x.
+Proof.
+  destruct x as [[] x]; unfold InvState.Unary.sem_idT in *; ss.
+  rewrite LOCALS_EQ; eauto.
+Qed.
+
+Lemma sem_valueT_eq_locals
+      conf st0 st1 invst0 v
+      (LOCALS_EQ: Locals (EC st0) = Locals (EC st1))
+  : InvState.Unary.sem_valueT conf st1 invst0 v = InvState.Unary.sem_valueT conf st0 invst0 v.
+Proof.
+  destruct v; eauto.
+  eapply sem_idT_eq_locals; eauto.
+Qed.
+
+Lemma sem_list_valueT_eq_locals
+      conf st0 st1 invst0 lsv
+      (LOCALS_EQ: Locals (EC st0) = Locals (EC st1))
+  : InvState.Unary.sem_list_valueT conf st1 invst0 lsv = InvState.Unary.sem_list_valueT conf st0 invst0 lsv.
+Proof.
+  induction lsv; ss; i.
+  destruct a as [s v].
+  exploit sem_valueT_eq_locals; eauto. intro EQ_VAL.
+  rewrite EQ_VAL. rewrite IHlsv. eauto.
+Qed.
+
+(* Lemma sem_expr_equiv_except_mem *)
+(*       conf st0 st1 invst0 invmem0 inv0 *)
+(*       (* cmd  *)mc def_memory e *)
+(*       (STATE : InvState.Unary.sem conf st0 invst0 invmem0 inv0) *)
+(*       (* (MEM_CHANGE : mem_change_cmd2 conf st0 mc cmd) *) *)
+(*       (* (DEF_MEM : Cmd.get_def_memory cmd = Some def_memory) *) *)
+(*       (MEM_EQUIV: state_equiv_except_mem conf st0 st1 mc) *)
+(*       (DEF_MEM_SEP: mem_change_noalias_expr mc e = true) *)
+(*       InvState.Unary.sem_valueT conf st0 invst0 *)
+(*       InvState. *)
+(*       Ptr.t *)
+(*                     (* Invariant.is_unique_ptr inv0 def_memory = true \/ *) *)
+(*                     (* ForgetMemory.is_noalias_Expr inv0 def_memory e = true) *) *)
+(*   : InvState.Unary.sem_expr conf st0 invst0 e = InvState.Unary.sem_expr conf st1 invst0 e. *)
+(* Proof. *)
+(*   ii. inv MEM_EQUIV. *)
+(*   destruct e; ss; *)
+(*     sem_value_st; eauto. *)
+(*   des_ifs. *)
+(*   destruct mc. *)
+(*   - inv MEM_CHANGE_EQUIV. *)
+(*     inv STATE. *)
+(*     des. *)
+(*     + unfold Invariant.is_unique_ptr in *. *)
+(*       unfold Invariant.is_unique_value in *. *)
+(*       destruct def_memory as [[[[] x]|] ty]; ss. *)
+(*       exploit UNIQUE. *)
+(*       { apply AtomSetFacts.mem_iff; eauto. } *)
+(*       i. *)
+(*       inv x0. *)
+
+(*       InvState.Unary.sem_noalias conf g _ t _ *)
+
+
+(* for same locals and memories *)
+Lemma sem_expr_eq_locals_mem
+      conf st0 st1 invst0 e
+      (LOCALS_EQ: Locals (EC st0) = Locals (EC st1))
+      (MEM_EQ: Mem st0 = Mem st1)
+  : InvState.Unary.sem_expr conf st1 invst0 e = InvState.Unary.sem_expr conf st0 invst0 e.
+Proof.
+  Ltac sem_value_st :=
+      let H' := fresh in
+      repeat
+        match goal with
+        | [LOCALS_EQ: Locals (EC ?st0) = Locals (EC ?st1) |-
+           context[ InvState.Unary.sem_valueT ?conf ?st1 ?invst0 ?v ] ] =>
+          exploit sem_valueT_eq_locals; try exact LOCALS_EQ; intro H';
+          rewrite H'; clear H'
+        | [LOCALS_EQ: Locals (EC ?st0) = Locals (EC ?st1) |-
+           context[ InvState.Unary.sem_list_valueT ?conf ?st1 ?invst0 ?lsv ] ] =>
+          exploit sem_list_valueT_eq_locals; try exact LOCALS_EQ; intro H';
+          rewrite H'; clear H'
+        end.
+  destruct e; ss; try rewrite <- MEM_EQ; sem_value_st; eauto.
+Qed.
+
+Lemma unary_sem_eq_locals_mem
+      conf st0 st1 invst0 invmem0 inv0
+      (LOCALS_EQ: Locals (EC st0) = Locals (EC st1))
+      (MEM_EQ : Mem st0 = Mem st1)
+  : <<SEM_ST0: InvState.Unary.sem conf st0 invst0 invmem0 inv0>> <->
+    <<SEM_ST1: InvState.Unary.sem conf st1 invst0 invmem0 inv0>>.
+Proof.
+  split; intro STATE.
+  { inv STATE.
+    econs.
+    - ii.
+      exploit LESSDEF; eauto.
+      { erewrite sem_expr_eq_locals_mem; eauto. }
+      i. des.
+      esplits; eauto.
+      erewrite sem_expr_eq_locals_mem; eauto.
+    - inv NOALIAS.
+      econs; i; [exploit DIFFBLOCK | exploit NOALIAS0]; eauto;
+        erewrite sem_valueT_eq_locals; eauto.
+    - ii. exploit UNIQUE; eauto. intro UNIQ_X. inv UNIQ_X.
+      econs; try rewrite <- LOCALS_EQ; try rewrite <- MEM_EQ; eauto.
+    - ii. exploit PRIVATE; eauto.
+      erewrite sem_idT_eq_locals; eauto.
+  }
+  { inv STATE.
+    econs.
+    - ii.
+      exploit LESSDEF; eauto.
+      { erewrite sem_expr_eq_locals_mem; eauto. }
+      i. des.
+      esplits; eauto.
+      erewrite sem_expr_eq_locals_mem; eauto.
+    - inv NOALIAS.
+      econs; i; [exploit DIFFBLOCK | exploit NOALIAS0]; eauto;
+        erewrite sem_valueT_eq_locals; eauto.
+    - ii. exploit UNIQUE; eauto. intro UNIQ_X. inv UNIQ_X.
+      econs; try rewrite  LOCALS_EQ; try rewrite MEM_EQ; eauto.
+    - ii. exploit PRIVATE; eauto.
+      erewrite sem_idT_eq_locals; eauto.
+  }
+Qed.
+
+(* soundness proof *)
+
+Lemma forget_memory_unary_sound1
+      conf st0 invst0 invmem0 inv0
+      cmd st1 public gmax mem_change def_memory
+      (STATE: InvState.Unary.sem conf st0 invst0 invmem0 inv0)
+      (DEF_MEM: Cmd.get_def_memory cmd = Some def_memory)
+      (MEM: InvMem.Unary.sem conf gmax public st0.(Mem) invmem0)
+      (MEM_EQUIV: state_equiv_except_mem conf st0 st1 mem_change)
+      (MEM_CHANGE: mem_change_cmd_after conf st0 mem_change cmd inv0)
+      (NO_PRIVATE_PARENT: mem_change_no_private_parent conf mem_change invmem0.(InvMem.Unary.private_parent))
+      (UNIQUE_PRSV: unique_preserved_mem conf st1 inv0)
+  : <<STATE_UNARY: InvState.Unary.sem conf st1 invst0 invmem0 (ForgetMemory.unary def_memory inv0)>> /\
+                   <<MEM_UNARY: InvMem.Unary.sem conf gmax public st1.(Mem) invmem0>>.
+Proof.
+  destruct mem_change;
+    try by (destruct cmd; ss; des; congruence).
+  - splits.
+    admit.
+    admit.
+    
+    
+    (* + econs. *)
+    (*   { ii. ss. unfold ForgetMemory.unary in *. *)
+    (*     exploit forget_memory_def_sep_mem; eauto. i. *)
+    (*     exploit sem_expr_equiv_except_mem; eauto. *)
+    (*     { instantiate (1:= (fst x)). *)
+    (*       des; try by left; eauto. *)
+    (*       right. unfold ForgetMemory.is_noalias_ExprPair in *. des_bool. des. ss. *)
+    (*     } *)
+    (*     exploit sem_expr_equiv_except_mem; eauto. *)
+    (*     { instantiate (1:= (snd x)). *)
+    (*       des; try by left; eauto. *)
+    (*       right. unfold ForgetMemory.is_noalias_ExprPair in *. des_bool. des. ss. *)
+    (*     } *)
+    (*     i. *)
+    (*     inv STATE. *)
+    (*     exploit LESSDEF. *)
+    (*     { des_ifs; eauto. *)
+    (*       ss. eapply ExprPairSetFacts.filter_iff in H; eauto; try by solve_compat_bool. inv H; eauto. *)
+    (*     } *)
+    (*     { rewrite x0. eauto. } *)
+    (*     i. rewrite <- x2. eauto. *)
+    (*   } *)
+    (*   { admit. (* alias *) } *)
+    (*   { admit. } *)
+    (*   { admit. } *)
+    (* + inv MEM_EQUIV. *)
+    (*   inv MEM_CHANGE_EQUIV. *)
+    (*   inv MEM. *)
+    (*   econs; eauto. *)
+    (*   { i. exploit PRIVATE; eauto. i. des. *)
+    (*     split; eauto. *)
+    (*     admit. (* nextblock preserved after mstore *) } *)
+    (*   { i. exploit PRIVATE_PARENT; eauto. i. des. *)
+    (*     split; eauto. *)
+    (*     admit. (* same *) } *)
+    (*   { unfold mem_change_no_private_parent in *. *)
+    (*     i. exploit MEM_PARENT; eauto. *)
+    (*     i. rewrite x. *)
+    (*     (* STORE: (Mem st1) = mstore (Mem st0) ptr .. *) *)
+    (*     (* mstore says GV2ptr ptr = Some Vptr .. *) *)
+    (*     (* NO_PRIVATE_PARENT tells us ~In b_ptr (private_parent) *) *)
+    (*     (* since b is In private_parent, mload_aux ?mem b should be preserved *) *)
+    (*     admit. *)
+    (*   } *)
+  
+  - admit. (* free case - almost same as above *)
+Admitted.
+
+Lemma forget_memory_unary_sound2
+      conf st0 st1 mem_change
+      cmd invst0 invmem0 inv0 gmax public
+      (STATE: InvState.Unary.sem conf st0 invst0 invmem0 inv0)
+      (DEF_MEM: Cmd.get_def_memory cmd = None)
+      (MEM: InvMem.Unary.sem conf gmax public st0.(Mem) invmem0)
+      (MEM_EQUIV : state_equiv_except_mem conf st0 st1 mem_change)
+      (MEM_CHANGE : mem_change_cmd_after conf st0 mem_change cmd inv0)
+      (NO_PRIVATE_PARENT: mem_change_no_private_parent conf mem_change invmem0.(InvMem.Unary.private_parent))
+      (UNIQUE_PRSV: unique_preserved_mem conf st1 inv0)
+  : <<STATE_UNARY: InvState.Unary.sem conf st1 invst0 invmem0 inv0>> /\
+    <<MEM_UNARY: InvMem.Unary.sem conf gmax public st1.(Mem) invmem0>>.
+Proof.
+  destruct mem_change.
+  - destruct cmd; ss.
+    + admit. (* TODO: doing here *)
+    + admit. (* exactly same as above *)
+  - destruct cmd; ss; des; congruence.
+  - destruct cmd; ss; des; congruence.
+  - inv MEM_EQUIV. inv STATES_MEM_CHANGE.
+    rewrite <- MEM_EQ.
+    esplits; eauto.
+    eapply unary_sem_eq_locals_mem; try (symmetry in LOCALS_EQ; exact LOCALS_EQ); eauto.
+Admitted.
+
+Lemma forget_memory_maydiff_preserved
+      conf_src st0_src st1_src mem_change_src def_mem_src
+      conf_tgt st0_tgt st1_tgt mem_change_tgt def_mem_tgt
+      invst0 invmem0 inv0
+      (MEM_EQUIV_SRC : state_equiv_except_mem conf_src st0_src st1_src mem_change_src)
+      (MEM_EQUIV_TGT : state_equiv_except_mem conf_tgt st0_tgt st1_tgt mem_change_tgt)
+      (MAYDIFF : forall id : Tag.t * id,
+          IdTSet.mem id (Invariant.maydiff inv0) = false ->
+          InvState.Rel.sem_inject st0_src st0_tgt invst0 (InvMem.Rel.inject invmem0) id)
+  : <<RES: forall id : Tag.t * id,
+      IdTSet.mem id (Invariant.maydiff (ForgetMemory.t def_mem_src def_mem_tgt inv0)) = false ->
+      InvState.Rel.sem_inject st1_src st1_tgt invst0 (InvMem.Rel.inject invmem0) id>>.
+Proof.
+  ii.
+  assert (DROP_FORGET_MEMORY:IdTSet.mem id0 (Invariant.maydiff inv0) = false).
+  { destruct def_mem_src; destruct def_mem_tgt; ss. }
+  exploit MAYDIFF; eauto.
+  { inv MEM_EQUIV_SRC.
+    unfold InvState.Unary.sem_idT in *.
+    destruct id0 as [[] x]; eauto.
+    ss. rewrite LOCALS_EQ. eauto.
+  }
+  i. des.
+  esplits; eauto.
+  inv MEM_EQUIV_TGT.
+  unfold InvState.Unary.sem_idT in *.
+  destruct id0 as [[] x]; eauto.
+  ss. rewrite <- LOCALS_EQ. eauto.
+Qed.
 
 Lemma some_injective A (a b:A):
   Some a = Some b -> a = b.
@@ -192,87 +521,15 @@ Proof.
   congruence.
 Qed.
 
-(* monotonic feature of ForgetMemory *)
-
-Lemma not_in_maydiff_forget_memory_monotone
-      def_mem_src def_mem_tgt inv0 v
-      (NOT_MD: Invariant.not_in_maydiff (ForgetMemory.t def_mem_src def_mem_tgt inv0) v = true)
-  : Invariant.not_in_maydiff inv0 v = true.
-Proof.
-  unfold Invariant.not_in_maydiff in *.
-  unfold ForgetMemory.t in *.
-  destruct def_mem_tgt; destruct def_mem_src; ss.
-Qed.
-
-Lemma ExprPairSet_forget_memory_monotone
-      ep def_mem inv0
-      (INJECT: ExprPairSet.mem ep (Invariant.lessdef (ForgetMemory.unary def_mem inv0)) = true)
-  : ExprPairSet.mem ep (Invariant.lessdef inv0) = true.
-Proof.
-  unfold ForgetMemory.unary in *.
-  des_ifs. ss.
-  rewrite ExprPairSetFacts.filter_b in *; try by solve_compat_bool.
-  rewrite andb_true_iff in *. des. eauto.
-Qed.
-
-Lemma inject_value_forget_memory_monotone
-      v1 def_mem_src
-      v2 def_mem_tgt
-      inv0
-      (INJECT: Invariant.inject_value
-                 (ForgetMemory.t def_mem_src def_mem_tgt inv0) v1 v2)
-  : Invariant.inject_value inv0 v1 v2.
-Proof.
-  unfold Invariant.inject_value in *.
-  unfold is_true in *.
-  repeat rewrite orb_true_iff in INJECT.
-  repeat rewrite orb_true_iff.
-  des.
-  - left. left. left.
-    solve_des_bool.
-    apply andb_true_iff; split; eauto using not_in_maydiff_forget_memory_monotone.
-  - left. left. right.
-    solve_des_bool.
-    apply andb_true_iff; split; eauto using not_in_maydiff_forget_memory_monotone.
-    destruct def_mem_src; destruct def_mem_tgt; ss;
-      eapply ExprPairSet_forget_memory_monotone; eauto.
-  - left. right.
-    solve_des_bool.
-    apply andb_true_iff; split; eauto using not_in_maydiff_forget_memory_monotone.
-    destruct def_mem_src; destruct def_mem_tgt; ss;
-      eapply ExprPairSet_forget_memory_monotone; eauto.
-  - right.
-    rewrite <- ExprPairSetFacts.exists_iff in *;try by solve_compat_bool.
-    unfold ExprPairSet.Exists in *. des.
-    apply InvState.get_rhs_in_spec in INJECT. des.
-    esplits.
-    + eapply InvState.get_rhs_in_spec2; eauto.
-      destruct def_mem_src; destruct def_mem_tgt; ss;
-        rewrite ExprPairSetFacts.mem_iff in *;
-        eapply ExprPairSet_forget_memory_monotone; eauto.
-    + solve_des_bool.
-      apply andb_true_iff.
-      split.
-      * destruct def_mem_src; destruct def_mem_tgt; ss;
-          rewrite ExprPairSetFacts.mem_iff in *;
-          eapply ExprPairSet_forget_memory_monotone; eauto.
-      * unfold Invariant.not_in_maydiff_expr in *.
-        apply forallb_forall. i.
-        eapply forallb_forall in INJECT2; eauto.
-        eapply not_in_maydiff_forget_memory_monotone; eauto.
-Qed.
-
-(* soundness *)
-
 Lemma mem_inject_change
-      conf_src mem0_src mem1_src mem_change_src
-      conf_tgt mem0_tgt mem1_tgt mem_change_tgt
+      conf_src st0_src st1_src mem_change_src
+      conf_tgt st0_tgt st1_tgt mem_change_tgt
       invmem0
-      (MEM_CHANGE_EQUIV_SRC : mem_change_equiv conf_src mem0_src mem1_src mem_change_src)
-      (MEM_CHANGE_EQUIV_TGT : mem_change_equiv conf_tgt mem0_tgt mem1_tgt mem_change_tgt)
+      (MEM_CHANGE_EQUIV_SRC : states_mem_change conf_src st0_src st1_src mem_change_src)
+      (MEM_CHANGE_EQUIV_TGT : states_mem_change conf_tgt st0_tgt st1_tgt mem_change_tgt)
       (MEM_CHANGE_INJECT : mem_change_inject conf_src conf_tgt invmem0 mem_change_src mem_change_tgt)
-      (INJECT : Memory.Mem.inject invmem0.(InvMem.Rel.inject) mem0_src mem0_tgt)
-  : Memory.Mem.inject invmem0.(InvMem.Rel.inject) mem1_src mem1_tgt.
+      (INJECT : Memory.Mem.inject invmem0.(InvMem.Rel.inject) st0_src.(Mem) st0_tgt.(Mem))
+  : Memory.Mem.inject invmem0.(InvMem.Rel.inject) st1_src.(Mem) st1_tgt.(Mem).
 Proof.
   inv MEM_CHANGE_INJECT.
   - inv INJECT. inv MEM_CHANGE_EQUIV_SRC. inv MEM_CHANGE_EQUIV_TGT.
@@ -309,6 +566,7 @@ Proof.
         hexploit Memory.Mem.fresh_block_alloc; try (symmetry; exact MALLOC); eauto. i.
         exploit mi_freeblocks; eauto. i. clarify.
   - inv INJECT. inv MEM_CHANGE_EQUIV_SRC. inv MEM_CHANGE_EQUIV_TGT.
+    rewrite <- MEM_EQ; clear MEM_EQ.
     unfold malloc in *.
     apply some_injective in MALLOC.
     econs.
@@ -339,6 +597,7 @@ Proof.
         hexploit Memory.Mem.fresh_block_alloc; try (symmetry; exact MALLOC); eauto. i.
         exploit mi_freeblocks; eauto. i. clarify.
   - inv INJECT. inv MEM_CHANGE_EQUIV_SRC. inv MEM_CHANGE_EQUIV_TGT.
+    rewrite <- MEM_EQ; clear MEM_EQ.
     unfold malloc in *.
     apply some_injective in MALLOC.
     econs.
@@ -368,199 +627,11 @@ Proof.
     eauto.
 Admitted.
 
-Lemma forget_memory_maydiff_preserved
-      conf_src st0_src st1_src mem_change_src def_mem_src
-      conf_tgt st0_tgt st1_tgt mem_change_tgt def_mem_tgt
-      invst0 invmem0 inv0
-      (MEM_EQUIV_SRC : state_equiv_except_mem conf_src st0_src st1_src mem_change_src)
-      (MEM_EQUIV_TGT : state_equiv_except_mem conf_tgt st0_tgt st1_tgt mem_change_tgt)
-      (MAYDIFF : forall id : Tag.t * id,
-          IdTSet.mem id (Invariant.maydiff inv0) = false ->
-          InvState.Rel.sem_inject st0_src st0_tgt invst0 (InvMem.Rel.inject invmem0) id)
-  : <<RES: forall id : Tag.t * id,
-      IdTSet.mem id (Invariant.maydiff (ForgetMemory.t def_mem_src def_mem_tgt inv0)) = false ->
-      InvState.Rel.sem_inject st1_src st1_tgt invst0 (InvMem.Rel.inject invmem0) id>>.
-Proof.
-  ii.
-  assert (DROP_FORGET_MEMORY:IdTSet.mem id0 (Invariant.maydiff inv0) = false).
-  { destruct def_mem_src; destruct def_mem_tgt; ss. }
-  exploit MAYDIFF; eauto.
-  { inv MEM_EQUIV_SRC.
-    unfold InvState.Unary.sem_idT in *.
-    destruct id0 as [[] x]; eauto.
-    ss. rewrite LOCALS_EQ. eauto.
-  }
-  i. des.
-  esplits; eauto.
-  inv MEM_EQUIV_TGT.
-  unfold InvState.Unary.sem_idT in *.
-  destruct id0 as [[] x]; eauto.
-  ss. rewrite <- LOCALS_EQ. eauto.
-Qed.
-
-Lemma sem_idT_eq_locals
-      st0 st1 invst0 x gv
-      (SEM_IDT: InvState.Unary.sem_idT st1 invst0 x = Some gv)
-      (LOCALS_EQ : Locals (EC st0) = Locals (EC st1))
-  : InvState.Unary.sem_idT st0 invst0 x = Some gv.
-Proof.
-  destruct x as [[] x]; unfold InvState.Unary.sem_idT in *; ss.
-  rewrite LOCALS_EQ; eauto.
-Qed.    
-
-Lemma sem_valueT_eq_locals
-      conf st0 st1 invst0 v gv
-      (SEM_EXPR: InvState.Unary.sem_valueT conf st0 invst0 v = Some gv)
-      (LOCALS_EQ: Locals (EC st0) = Locals (EC st1))
-  : InvState.Unary.sem_valueT conf st1 invst0 v = Some gv.
-Proof.
-  destruct v; eauto.
-  eapply sem_idT_eq_locals; eauto.
-Qed.
-
-Lemma sem_list_valueT_eq_locals
-      conf st0 st1 invst0 lsv lgv
-      (SEM_EXPR: InvState.Unary.sem_list_valueT conf st0 invst0 lsv = Some lgv)
-      (LOCALS_EQ: Locals (EC st0) = Locals (EC st1))
-  : InvState.Unary.sem_list_valueT conf st1 invst0 lsv = Some lgv.
-Proof.
-  revert lgv SEM_EXPR.
-  induction lsv; ss; i.
-  des_ifs.
-  - exploit IHlsv; eauto. i.
-    symmetry in LOCALS_EQ.
-    exploit sem_valueT_eq_locals; eauto. i. clarify.
-  - exploit IHlsv; eauto. i.
-    clarify.
-  - exploit sem_valueT_eq_locals; eauto. i. clarify.
-Qed.
-
-Ltac sem_valueT_congruence :=
-      repeat
-        match goal with
-        | [H1: InvState.Unary.sem_valueT ?conf ?st1 ?invst ?v = Some ?gv1,
-               H2: InvState.Unary.sem_valueT ?conf ?st2 ?invst ?v = _,
-                   LOCALS: Locals (EC ?st1) = Locals (EC ?st2) |- _] =>
-          erewrite sem_valueT_eq_locals in H2; try exact H1; try exact LOCALS; inv H2
-        | [H1: InvState.Unary.sem_list_valueT ?conf ?st1 ?invst ?lsv = Some ?lgv,
-               H2: InvState.Unary.sem_list_valueT ?conf ?st2 ?invst ?lsv = _,
-                   LOCALS: Locals (EC ?st1) = Locals (EC ?st2) |- _] =>
-          erewrite sem_list_valueT_eq_locals in H2; try exact H1; try exact LOCALS; inv H2
-        end;
-      eauto; try congruence.
-
-Lemma sem_expr_eq_locals_mem
-      conf st0 st1 invst0 e gv
-      (SEM_EXPR: InvState.Unary.sem_expr conf st0 invst0 e = Some gv)
-      (LOCALS_EQ: Locals (EC st0) = Locals (EC st1))
-      (MEM_EQ: Mem st0 = Mem st1)
-  : InvState.Unary.sem_expr conf st1 invst0 e = Some gv.
-Proof.
-  destruct e; ss;
-    des_ifs; sem_valueT_congruence; clarify.
-  eapply sem_valueT_eq_locals; eauto.
-Qed.
-
-Lemma unary_sem_eq_locals_mem
-      conf st0 st1 invst0 invmem0 inv0
-      (STATE: InvState.Unary.sem conf st0 invst0 invmem0 inv0)
-      (LOCALS_EQ: Locals (EC st0) = Locals (EC st1))
-      (MEM_EQ : Mem st0 = Mem st1)
-  : InvState.Unary.sem conf st1 invst0 invmem0 inv0.
-Proof.
-  inv STATE.
-  econs.
-  - ii.
-    exploit LESSDEF; eauto.
-    { eapply sem_expr_eq_locals_mem; eauto. }
-    i. des.
-    esplits; eauto.
-    exploit sem_expr_eq_locals_mem; eauto.
-  - inv NOALIAS.
-    econs; i; [exploit DIFFBLOCK | exploit NOALIAS0]; eauto;
-      eapply sem_valueT_eq_locals; eauto.
-  - ii. exploit UNIQUE; eauto. intro UNIQ_X. inv UNIQ_X.
-    econs; try rewrite <- LOCALS_EQ; try rewrite <- MEM_EQ; eauto.
-  - ii. exploit PRIVATE; eauto.
-    eapply sem_idT_eq_locals; eauto.
-Qed.
-
-Lemma forget_memory_unary_sound1
-      conf st0 invst0 invmem0 inv0
-      cmd st1 public gmax mem_change def_memory
-      (STATE: InvState.Unary.sem conf st0 invst0 invmem0 inv0)
-      (DEF_MEM: Cmd.get_def_memory cmd = Some def_memory)
-      (MEM: InvMem.Unary.sem conf gmax public st0.(Mem) invmem0)
-      (MEM_EQUIV: state_equiv_except_mem conf st0 st1 mem_change)
-      (MEM_CHANGE: mem_change_rel2 conf st0 mem_change cmd)
-      (UNIQUE_PRSV: unique_preserved_mem conf st1 inv0)
-  : <<STATE_UNARY: InvState.Unary.sem conf st1 invst0 invmem0 (ForgetMemory.unary def_memory inv0)>> /\
-                   <<MEM_UNARY: InvMem.Unary.sem conf gmax public st1.(Mem) invmem0>>.
-Proof.
-  destruct mem_change;
-    try by (destruct cmd; ss; des; congruence).
-  - splits.
-    + inv STATE.
-      (* econs; eauto. *)
-      (* { ii. exploit LESSDEF; eauto. *)
-      admit. (* lessdef - should treat load *)
-    + inv MEM_EQUIV.
-      inv MEM_CHANGE_EQUIV.
-      inv MEM.
-      admit. (* mstore, mstore_aux *)
-  - splits.
-    + inv STATE.
-      (* econs. *)
-      (* { ii. *)
-      (*   exploit LESSDEF. *)
-      (*   { admit. (* in - monotone *) } *)
-      (*   { admit. (* sem_expr monotone? *) } *)
-      (*   i. des. *)
-      (*   esplits; eauto. *)
-      (*   admit. *)
-      (* } *)
-      admit.
-    + inv MEM_EQUIV.
-      inv MEM_CHANGE_EQUIV.
-      inv MEM.
-      unfold free in *. des_ifs.
-      econs; eauto.
-      * i. exploit PRIVATE; eauto. i. des.
-        split; eauto.
-        exploit Memory.Mem.valid_block_free_1; eauto.
-      * i. exploit PRIVATE_PARENT; eauto. i. des.
-        split; eauto.
-        exploit Memory.Mem.valid_block_free_1; eauto.
-      *  i. exploit MEM_PARENT; eauto.
-         admit. (* should handle mload_aux *)
-Admitted.
-
-Lemma forget_memory_unary_sound2
-      conf st0 st1 mem_change
-      cmd invst0 invmem0 inv0 gmax public
-      (STATE: InvState.Unary.sem conf st0 invst0 invmem0 inv0)
-      (DEF_MEM: Cmd.get_def_memory cmd = None)
-      (MEM: InvMem.Unary.sem conf gmax public st0.(Mem) invmem0)
-      (MEM_EQUIV : state_equiv_except_mem conf st0 st1 mem_change)
-      (MEM_CHANGE : mem_change_rel2 conf st0 mem_change cmd)
-      (UNIQUE_PRSV: unique_preserved_mem conf st1 inv0)
-  : <<STATE_UNARY: InvState.Unary.sem conf st1 invst0 invmem0 inv0>> /\
-    <<MEM_UNARY: InvMem.Unary.sem conf gmax public st1.(Mem) invmem0>>.
-Proof.
-  destruct mem_change.
-  - admit.
-  - destruct cmd; ss; des; congruence.
-  - destruct cmd; ss; des; congruence.
-  - inv MEM_EQUIV. inv MEM_CHANGE_EQUIV.
-    rewrite <- MEM_EQ.
-    esplits; eauto.
-    eapply unary_sem_eq_locals_mem; eauto.
-Admitted.
-
 Lemma forget_memory_sound
-      conf_src st0_src st1_src mem_change_src cmd_src
-      conf_tgt st0_tgt st1_tgt mem_change_tgt cmd_tgt
+      m_src conf_src st0_src st1_src mem_change_src cmd_src
+      m_tgt conf_tgt st0_tgt st1_tgt mem_change_tgt cmd_tgt
       invst0 invmem0 inv0
+      (CONF: InvState.valid_conf m_src m_tgt conf_src conf_tgt)
       (STATE: InvState.Rel.sem conf_src conf_tgt st0_src st0_tgt invst0 invmem0 inv0)
       (MEM: InvMem.Rel.sem conf_src conf_tgt st0_src.(Mem) st0_tgt.(Mem) invmem0)
       (MEM_EQUIV_SRC: state_equiv_except_mem
@@ -571,8 +642,8 @@ Lemma forget_memory_sound
                         conf_tgt
                         st0_tgt st1_tgt
                         mem_change_tgt)
-      (MEM_CHANGE_SRC: mem_change_rel2 conf_src st0_src mem_change_src cmd_src)
-      (MEM_CHANGE_TGT: mem_change_rel2 conf_tgt st0_tgt mem_change_tgt cmd_tgt)
+      (MEM_CHANGE_SRC: mem_change_cmd_after conf_src st0_src mem_change_src cmd_src inv0.(Invariant.src))
+      (MEM_CHANGE_TGT: mem_change_cmd_after conf_tgt st0_tgt mem_change_tgt cmd_tgt inv0.(Invariant.tgt))
       (MEM_CHANGE_INJECT: mem_change_inject conf_src conf_tgt invmem0 mem_change_src mem_change_tgt)
       (UNIQUE_PRSV_SRC: unique_preserved_mem conf_src st1_src inv0.(Invariant.src))
       (UNIQUE_PRSV_TGT: unique_preserved_mem conf_tgt st1_tgt inv0.(Invariant.tgt))
@@ -580,8 +651,10 @@ Lemma forget_memory_sound
                               (ForgetMemory.t (Cmd.get_def_memory cmd_src) (Cmd.get_def_memory cmd_tgt) inv0) >> /\
     <<MEM: InvMem.Rel.sem conf_src conf_tgt st1_src.(Mem) st1_tgt.(Mem) invmem0>>.
 Proof.
+  exploit mem_change_inject_no_private_parent_src; eauto. intro NO_PRIVATE_PARENT_SRC.
+  exploit mem_change_inject_no_private_parent_tgt; eauto. intro NO_PRIVATE_PARENT_TGT.
   inv STATE. inv MEM.
-  
+
   destruct (Cmd.get_def_memory cmd_src) eqn:DEF_MEM_SRC;
     destruct (Cmd.get_def_memory cmd_tgt) eqn:DEF_MEM_TGT.
   - hexploit forget_memory_unary_sound1; try exact SRC; try exact DEF_MEM_SRC; eauto. i. des.
@@ -609,142 +682,3 @@ Proof.
     hexploit mem_inject_change; try exact MEM_CHANGE_INJECT; eauto. i.
     esplits; econs; eauto.
 Qed.
-    
-(*     esplits. *)
-(*     + econs; eauto. *)
-(*       ss. i. *)
-(*       hexploit MAYDIFF; eauto. i. *)
-(*       ii. *)
-(*       i. *)
-(*       ss. eauto. *)
-(*       admit. *)
-(*     + econs; eauto. *)
-(*       eapply mem_inject_change; eauto. *)
-(*       * inv MEM_EQUIV_SRC; eauto. *)
-(*       * inv MEM_EQUIV_TGT; eauto. *)
-(*   - *)
-  
-(*   inv STATE. *)
-(*   destruct mem_change_src; destruct mem_change_tgt; inv MEM_CHANGE_INJECT. *)
-(*   - destruct cmd_src eqn:CMDSRC; destruct cmd_tgt eqn:CMDTGT; ss; des; *)
-(*       try congruence. *)
-(*     + inv MEM_CH; inv MEM_CH0. *)
-(*     +  *)
-
-(*     admit. (* alloc - alloc *) } *)
-(*   { admit. (* alloc - none *) } *)
-(*   { admit. (* store - store *) } *)
-(*   { admit. (* store - none *) } *)
-(*   { admit. (* free - free *) } *)
-(*   { admit. (* none - alloc *) } *)
-(*   { admit. (* none - none *) } *)
-
-
-  
-(*   destruct (Cmd.get_def_memory cmd_src) eqn:DEF_MEM_SRC; *)
-(*     destruct (Cmd.get_def_memory cmd_tgt) eqn:DEF_MEM_TGT. *)
-(*   - destruct cmd_src; destruct cmd_tgt; ss. *)
-(*     + admit. (* free - free *) *)
-(*     + admit. (* free - store : cont. *) *)
-(*     + admit. (* store - free : cont.  *) *)
-(*     + admit. (* store - store *) *)
-(*   - (* destruct cmd_src; destruct cmd_tgt; ss. *) *)
-(*     admit. *)
-(*   - admit. *)
-(*   - ss. *)
-(*     unfold mem_change_rel2 in *. *)
-(*     destruct cmd_src; destruct cmd_tgt; ss. *)
-
-
-
-
-  
-(*   unfold ForgetMemory.t. *)
-(*   destruct def_memory_src as [[]|], def_memory_tgt as [[]|]; ss. *)
-(*   inv MEM. *)
-
-(*   - exploit forget_memory_unary_sound1; try exact SRC; eauto. i. des. *)
-(*     exploit forget_memory_unary_sound1; try exact TGT; eauto. i. des. *)
-(*     splits. *)
-(*     + econs; ss; eauto. i. *)
-(*       hexploit MAYDIFF; eauto. i. *)
-(*       ii. exploit H. *)
-(*       { destruct id0 as [[]]; eauto. *)
-(*         inv MEM_EQUIV_SRC; solve_sem_idT. *)
-(*         rewrite -> LOCALS_EQ; eauto. *)
-(*       } *)
-(*       i. des. *)
-(*       esplits; eauto. *)
-(*       destruct id0 as [[]]; eauto. *)
-(*       inv MEM_EQUIV_TGT; *)
-(*         solve_sem_idT; rewrite <- LOCALS_EQ; eauto. *)
-(*     + econs; ss; eauto. *)
-(*       inv MEM_EQUIV_SRC. *)
-(*       inv MEM_EQUIV_TGT. *)
-
-(*       eapply mem_inject_change; eauto. *)
-      
-(*   - inv MEM. *)
-(*     exploit forget_memory_unary_sound1; try exact SRC; eauto. i. des. *)
-(*     exploit forget_memory_unary_sound2; try exact TGT; eauto. i. des. *)
-(*     splits. *)
-(*     + econs; ss; eauto. *)
-(*       i. *)
-(*       hexploit MAYDIFF; eauto. i. *)
-(*       ii. exploit H. *)
-(*       { destruct id0 as [[]]; eauto. *)
-(*         inv MEM_EQUIV_SRC; solve_sem_idT. *)
-(*         rewrite -> LOCALS_EQ; eauto. *)
-(*       } *)
-(*       i. des. *)
-(*       esplits; eauto. *)
-(*       destruct id0 as [[]]; eauto. *)
-(*       inv MEM_EQUIV_TGT; *)
-(*         solve_sem_idT; rewrite <- LOCALS_EQ; eauto. *)
-(*     + econs; ss; eauto. *)
-(*       inv MEM_EQUIV_SRC. *)
-(*       inv MEM_EQUIV_TGT. *)
-(*       eapply mem_inject_change; eauto. *)
-(*   - inv MEM. *)
-(*     exploit forget_memory_unary_sound2; try exact SRC; eauto. i. des. *)
-(*     exploit forget_memory_unary_sound1; try exact TGT; eauto. i. des. *)
-(*     splits. *)
-(*     + econs; ss; eauto. *)
-(*       i. *)
-(*       hexploit MAYDIFF; eauto. i. *)
-(*       ii. exploit H. *)
-(*       { destruct id0 as [[]]; eauto. *)
-(*         inv MEM_EQUIV_SRC; solve_sem_idT. *)
-(*         rewrite -> LOCALS_EQ; eauto. *)
-(*       } *)
-(*       i. des. *)
-(*       esplits; eauto. *)
-(*       destruct id0 as [[]]; eauto. *)
-(*       inv MEM_EQUIV_TGT; *)
-(*         solve_sem_idT; rewrite <- LOCALS_EQ; eauto. *)
-(*     + econs; ss; eauto. *)
-(*       inv MEM_EQUIV_SRC. *)
-(*       inv MEM_EQUIV_TGT. *)
-(*       eapply mem_inject_change; eauto. *)
-(*   - inv MEM. *)
-(*     exploit forget_memory_unary_sound2; try exact SRC; eauto. i. des. *)
-(*     exploit forget_memory_unary_sound2; try exact TGT; eauto. i. des. *)
-(*     splits. *)
-(*     + econs; ss; eauto. *)
-(*       i. *)
-(*       hexploit MAYDIFF; eauto. i. *)
-(*       ii. exploit H. *)
-(*       { destruct id0 as [[]]; eauto. *)
-(*         inv MEM_EQUIV_SRC; solve_sem_idT. *)
-(*         rewrite -> LOCALS_EQ; eauto. *)
-(*       } *)
-(*       i. des. *)
-(*       esplits; eauto. *)
-(*       destruct id0 as [[]]; eauto. *)
-(*       inv MEM_EQUIV_TGT; *)
-(*         solve_sem_idT; rewrite <- LOCALS_EQ; eauto. *)
-(*     + econs; ss; eauto. *)
-(*       inv MEM_EQUIV_SRC. *)
-(*       inv MEM_EQUIV_TGT. *)
-(*       eapply mem_inject_change; eauto. *)
-(* Admitted. *)
